src/riscv/Proofs/InstructionSetOrder.v
@@ -9,52 +9,64 @@ Record InstructionSet': Set := {
   supports_M: bool;
   supports_A: bool;
   supports_F: bool;
+  supports_V: bool
 }.
 
-Definition toInstructionSet(i: InstructionSet'): InstructionSet :=
-  match i.(supports_64bit), i.(supports_M), i.(supports_A), i.(supports_F) with
-  | false, false, false, false => RV32I
-  | false, false, false, true  => RV32IF
-  | false, false, true , false => RV32IA
-  | false, false, true , true  => RV32IAF
-  | false, true , false, false => RV32IM
-  | false, true , false, true  => RV32IMF
-  | false, true , true , false => RV32IMA
-  | false, true , true , true  => RV32IMAF
-  | true , false, false, false => RV64I
-  | true , false, false, true  => RV64IF
-  | true , false, true , false => RV64IA
-  | true , false, true , true  => RV64IAF
-  | true , true , false, false => RV64IM
-  | true , true , false, true  => RV64IMF
-  | true , true , true , false => RV64IMA
-  | true , true , true , true  => RV64IMAF
+Definition toInstructionSet(i: InstructionSet'): option InstructionSet :=
+  match i.(supports_64bit), i.(supports_M), i.(supports_A), i.(supports_F), i.(supports_V) with
+  | false, false, false, false, false => Some RV32I
+  | false, false, false, true, false  => Some RV32IF
+  | false, false, true , false, false => Some RV32IA
+  | false, false, true , true, false  => Some RV32IAF
+  | false, true , false, false, false => Some RV32IM
+  | false, true , false, true, false  => Some RV32IMF
+  | false, true , true , false, false => Some RV32IMA
+  | false, true , true , true, false  => Some RV32IMAF
+  | true , false, false, false, false => Some RV64I
+  | true , false, false, true, false  => Some RV64IF
+  | true , false, true , false, false => Some RV64IA
+  | true , false, true , true, false  => Some RV64IAF
+  | true , true , false, false, false => Some RV64IM
+  | true , true , false, true, false  => Some RV64IMF
+  | true , true , true , false, false => Some RV64IMA
+  | true , true , true , true, false  => Some RV64IMAF
+  | true, true, false, false, true => Some RV64IMV
+  | _, _, _, _, _ => None
   end.
 
 Definition fromInstructionSet(i: InstructionSet): InstructionSet' :=
   match i with
-  | RV32I    => Build_InstructionSet' false false false false
-  | RV32IF   => Build_InstructionSet' false false false true
-  | RV32IA   => Build_InstructionSet' false false true  false
-  | RV32IAF  => Build_InstructionSet' false false true  true
-  | RV32IM   => Build_InstructionSet' false true  false false
-  | RV32IMF  => Build_InstructionSet' false true  false true
-  | RV32IMA  => Build_InstructionSet' false true  true  false
-  | RV32IMAF => Build_InstructionSet' false true  true  true
-  | RV64I    => Build_InstructionSet' true  false false false
-  | RV64IF   => Build_InstructionSet' true  false false true
-  | RV64IA   => Build_InstructionSet' true  false true  false
-  | RV64IAF  => Build_InstructionSet' true  false true  true
-  | RV64IM   => Build_InstructionSet' true  true  false false
-  | RV64IMF  => Build_InstructionSet' true  true  false true
-  | RV64IMA  => Build_InstructionSet' true  true  true  false
-  | RV64IMAF => Build_InstructionSet' true  true  true  true
+  | RV32I    => Build_InstructionSet' false false false false false
+  | RV32IF   => Build_InstructionSet' false false false true  false
+  | RV32IA   => Build_InstructionSet' false false true  false false
+  | RV32IAF  => Build_InstructionSet' false false true  true  false
+  | RV32IM   => Build_InstructionSet' false true  false false false
+  | RV32IMF  => Build_InstructionSet' false true  false true  false
+  | RV32IMA  => Build_InstructionSet' false true  true  false false
+  | RV32IMAF => Build_InstructionSet' false true  true  true  false
+  | RV64I    => Build_InstructionSet' true  false false false false
+  | RV64IF   => Build_InstructionSet' true  false false true  false
+  | RV64IA   => Build_InstructionSet' true  false true  false false
+  | RV64IAF  => Build_InstructionSet' true  false true  true  false
+  | RV64IM   => Build_InstructionSet' true  true  false false false
+  | RV64IMF  => Build_InstructionSet' true  true  false true  false
+  | RV64IMA  => Build_InstructionSet' true  true  true  false false
+  | RV64IMAF => Build_InstructionSet' true  true  true  true  false
+  | RV64IMV  => Build_InstructionSet' true  true  false false true
   end.
 
-Lemma from_toInstructionSet: forall i, fromInstructionSet (toInstructionSet i) = i.
-Proof. destruct i as [[|] [|] [|] [|]]; reflexivity. Qed.
+Lemma from_toInstructionSet: forall i, (i.(supports_V) = false) -> forall t, toInstructionSet i = Some t -> fromInstructionSet t = i.
+Proof. intros. unfold toInstructionSet in *.
+       all: destruct (supports_64bit i) eqn:E1; destruct (supports_M i) eqn:E2;
+         destruct (supports_A i) eqn:E3; destruct (supports_F i) eqn:E4; destruct (supports_V i) eqn:E5.
+       all: try solve [discriminate].
+       all: inversion H0; simpl.
+       all: destruct i.
+       all: unfold supports_64bit, supports_M, supports_A, supports_F, supports_V in *.
+       all: rewrite E1, E2, E3, E4, E5; reflexivity.
+Qed.
 
-Lemma to_fromInstructionSet: forall i, toInstructionSet (fromInstructionSet i) = i.
+Lemma to_fromInstructionSet: forall i, ((i = RV64IMV) -> False) -> toInstructionSet (fromInstructionSet i) = Some i.
 Proof. destruct i; reflexivity. Qed.
 
 Definition InstructionSet'_le(i1 i2: InstructionSet'): Prop :=
@@ -94,13 +106,14 @@ Qed.
 Lemma verify_iset_monotone: forall iset1 iset2 inst,
     InstructionSet'_le (fromInstructionSet iset1) (fromInstructionSet iset2) ->
     supportsF iset2 = false -> (* because verify_inst/decode_encode proofs don't support it yet *)
+    supportsV iset2 = false ->
     verify_iset inst iset1 ->
     verify_iset inst iset2.
 Proof.
   unfold verify_iset, InstructionSet'_le, Bool.le. destruct inst; auto.
-  all: intros (L1 & L2 & L3 & L4) SF C.
+  all: intros (L1 & L2 & L3 & L4) SF SV C.
   all: repeat match type of C with
-              | _ \/ _ => destruct C as [? | C]
+             | _ \/ _ => destruct C as [? | C]
               end;
     subst; cbn in *.
   all: destruct iset2; cbn in *; try intuition congruence.
@@ -109,6 +122,7 @@ Qed.
 Lemma verify_monotone: forall iset1 iset2 inst,
     InstructionSet'_le (fromInstructionSet iset1) (fromInstructionSet iset2) ->
     supportsF iset2 = false -> (* because verify_inst/decode_encode proofs don't support it yet *)
+    supportsV iset2 = false ->
     verify inst iset1 ->
     verify inst iset2.
 Proof.
